proof/Russell/Injectivity.v
@@ -1,3 +1,4 @@
+Require Import Lambda.Tactics.
 Require Import Lambda.Terms.
 Require Import Lambda.Reduction.
 Require Import Lambda.Conv.
@@ -11,6 +12,8 @@ Require Import Lambda.Russell.GenerationNotKind.
 Require Import Lambda.Russell.GenerationCoerce.
 Require Import Lambda.Russell.Generation.
 
+Require Import Lambda.Meta.Russell_TPOSR.
+
 Implicit Types i k m n p : nat.
 Implicit Type s : sort.
 Implicit Types A B M N T t u v : term.
@@ -18,7 +21,10 @@ Implicit Types e f g : env.
 
 Set Implicit Arguments.
 
-Axiom unique_sort_conv : forall G A A' s1 s2, G |-- A : Srt s1 -> G |-- A' : Srt s2 -> conv A A' -> s1 = s2.
+Lemma unique_sort_conv : forall G A A' s1 s2, G |-- A : Srt s1 -> G |-- A' : Srt s2 -> conv A A' -> s1 = s2.
+Proof.
+  apply russell_unique_sort_conv.
+Qed.
 
 Lemma inv_conv_prod_sort_l : forall e U V U' V' s, e |-- Prod U V : Srt s -> e |-- Prod U' V' : Srt s ->
   conv (Prod U V) (Prod U' V') -> exists s1 : sort, e |-- U : Srt s1 /\ e |-- U' : Srt s1 .
@@ -73,23 +79,47 @@ Proof.
   apply wf_var with s ; auto with coc.
 Qed.
 
-(** Set versions of the lemmas derived from the axiom *)
-Axiom inv_conv_prod_sort_l_set : forall e U V U' V' s, e |-- Prod U V : Srt s -> e |-- Prod U' V' : Srt s ->
-  conv (Prod U V) (Prod U' V') -> { s1 : sort | e |-- U : Srt s1 /\ e |-- U' : Srt s1 }.
+Require Import Lambda.Russell.UnicityOfSorting.
+
+(** Versions of the lemmas usable when in Set *)
+Lemma inv_conv_prod_sort_l_set : forall e U V U' V' s, 
+  e |-- Prod U V : Srt s -> e |-- Prod U' V' : Srt s ->
+  conv (Prod U V) (Prod U' V') -> 
+  forall s1, e |-- U : Srt s1 -> e |-- U' : Srt s1.
+Proof.
+  intros.
+  destruct (inv_conv_prod_sort_l H H0 H1).
+  destruct_exists.
+  rewrite (unique_sort H2 H3) ; auto.
+Qed.
 
 
-Axiom inv_conv_prod_sort_r_set : forall e U V U' V' s, e |-- Prod U V : Srt s -> e |-- Prod U' V' : Srt s ->
-  conv (Prod U V) (Prod U' V') -> U' :: e |-- V : Srt s /\ U' :: e |-- V' : Srt s. 
+Lemma inv_conv_prod_sort_r_set : forall e U V U' V' s, 
+  e |-- Prod U V : Srt s -> e |-- Prod U' V' : Srt s ->
+  conv (Prod U V) (Prod U' V') -> 
+  U' :: e |-- V : Srt s /\ U' :: e |-- V' : Srt s. 
+Proof.
+  intros.
+  destruct (inv_conv_prod_sort_r H H0 H1).
+  intuition.
+Qed.
 
-Axiom inv_conv_sum_sort_set : forall e U V U' V' s, e |-- Sum U V : Srt s -> e |-- Sum U' V' : Srt s ->
+Lemma inv_conv_sum_sort_l_set : forall e U V U' V' s, e |-- Sum U V : Srt s -> e |-- Sum U' V' : Srt s ->
   conv (Sum U V) (Sum U' V') -> 
-  { s1 : sort & { s2 : sort | e |-- U : Srt s1 /\ e |-- U' : Srt s1 /\ U :: e |-- V : Srt s2 /\ U :: e |-- V' : Srt s2
-  /\ sum_sort s1 s2 s}}.	
+  forall s1 : sort, e |-- U : Srt s1 -> e |-- U' : Srt s1.
+Proof.
+  intros.
+  destruct (inv_conv_sum_sort H H0 H1).
+  destruct_exists.
+  rewrite (unique_sort H2 H3) ; auto.
+Qed.
 
-Axiom inv_conv_sum_sort_l_set : forall e U V U' V' s, e |-- Sum U V : Srt s -> e |-- Sum U' V' : Srt s ->
+Lemma inv_conv_sum_sort_r_set : forall e U V U' V' s, e |-- Sum U V : Srt s -> e |-- Sum U' V' : Srt s ->
   conv (Sum U V) (Sum U' V') -> 
-  { s1 : sort | e |-- U : Srt s1 /\ e |-- U' : Srt s1 }.
-
-Axiom inv_conv_sum_sort_r_set : forall e U V U' V' s, e |-- Sum U V : Srt s -> e |-- Sum U' V' : Srt s ->
-  conv (Sum U V) (Sum U' V') -> 
-  { s2 : sort | U :: e |-- V : Srt s2 /\ U :: e |-- V' : Srt s2 }.
+  forall s2 : sort, U :: e |-- V : Srt s2 -> U :: e |-- V' : Srt s2.
+Proof.
+  intros.
+  destruct (inv_conv_sum_sort H H0 H1).
+  destruct_exists.
+  rewrite (unique_sort H2 H5) ; auto.
+Qed.
